utils.v
@@ -30,6 +30,24 @@ Section measure_rect.
 
 End measure_rect.
 
+Section length_split.
+
+  Variable (X : Type).
+  Implicit Type (ll : list X).
+
+  Fact list_length_split n ll : { l : _ & { r | ll = l++r /\ length l = n } } + { length ll < n }.
+  Proof.
+    revert ll; induction n as [ | n IHn ].
+    + left; exists nil, ll; auto.
+    + intros [ | x ll ].
+      * right; simpl; omega.
+      * destruct (IHn ll) as [ (l & r & H1 & H2) | H1 ].
+        - left; exists (x::l), r; split; subst; auto.
+        - right; simpl; omega.
+  Qed.
+
+End length_split.
+
 Section zip.
 
   Variable (X : Type) (f : X -> X -> X).
@@ -43,6 +61,25 @@ Section zip.
 
   Fact zip_fix_1 l : zip l nil = l.
   Proof. destruct l; auto. Qed.
+
+  Fact zip_app l1 l2 m1 m2 : length l1 = length m1 -> zip (l1++l2) (m1++m2) = zip l1 m1 ++ zip l2 m2.
+  Proof.
+    revert m1; induction l1 as [| ? ? IH]; intros [|]; simpl; auto; try discriminate; intros; f_equal; apply IH; omega.
+  Qed.
+
+  Fact zip_app_left l1 l2 m x : length m < length l1 -> In x l2 -> In x (zip (l1++l2) m).
+  Proof.
+    revert m; induction l1 as [ | y l1 IH ]; intros [ | z m ]; simpl; try omega.
+    + right; apply in_or_app; simpl; auto.
+    + intros H1 H2; right; apply IH; auto; omega.
+  Qed.
+
+  Fact zip_app_right l m1 m2 x : length l < length m1 -> In x m2 -> In x (zip l (m1++m2)).
+  Proof.
+    revert m1; induction l as [ | y l IH ]; intros [ | z m1 ]; simpl; try omega.
+    + right; apply in_or_app; simpl; auto.
+    + intros H1 H2; right; apply IH; auto; omega.
+  Qed.
 
   Fact zip_spec l m c : In c (zip l m) <-> (exists m1 m2, length l <= length m1 /\ m = m1++c::m2)
                                         \/ (exists l1 l2, length m <= length l1 /\ l = l1++c::l2)
